coq/ExpMap.v
@@ -1,4 +1,48 @@
-Load Exp.
+Load Core.
+
+Scheme le_sort_mono_ind' := Minimality for le_sort Sort Prop
+  with le_subst_mono_ind' := Minimality for le_subst Sort Prop
+  with le_term_mono_ind' := Minimality for le_term Sort Prop
+  with le_ctx_mono_ind' := Minimality for le_ctx Sort Prop
+  with le_ctx_var_mono_ind' := Minimality for le_ctx_var Sort Prop
+  with wf_sort_mono_ind' := Minimality for wf_sort Sort Prop
+  with wf_subst_mono_ind' := Minimality for wf_subst Sort Prop
+  with wf_term_mono_ind' := Minimality for wf_term Sort Prop
+  with wf_ctx_mono_ind' := Minimality for wf_ctx Sort Prop
+  with wf_ctx_var_mono_ind' := Minimality for wf_ctx_var Sort Prop
+  with wf_rule_ind' := Minimality for wf_rule Sort Prop
+  with wf_lang_ind' := Minimality for wf_lang Sort Prop.
+
+Combined Scheme mono_ind' from
+         le_sort_mono_ind',
+         le_subst_mono_ind',
+         le_term_mono_ind',
+         le_ctx_mono_ind',
+         le_ctx_var_mono_ind',
+         wf_sort_mono_ind',
+         wf_subst_mono_ind',
+         wf_term_mono_ind',
+         wf_ctx_mono_ind',
+         wf_ctx_var_mono_ind',
+         wf_rule_ind',
+         wf_lang_ind'.
+
+(*TODO: finish and put in the right place *)
+Lemma empty_subst_id {p} (e : exp p) : e[/[::]/] = e.
+Proof.
+  elim: e; auto.
+  intros.
+  simpl.
+  f_equal.
+  elim: v H; auto.
+  intros.
+  simpl.
+  inversion H0.
+  rewrite H.
+  rewrite H1.
+  auto.
+  assumption.
+Qed.
 
 Section Morphisms.
   
@@ -14,7 +58,128 @@ Section Morphisms.
     
     Definition morph_fn := alg_fn morph_alg.
     
+    Definition ctx_fn := List.map (ctx_var_map morph_fn).
+    
     Definition lang_fn := List.map (rule_map morph_fn).
+
+    Lemma morph_rule_in (l : lang p1) r : List.In r l -> List.In (rule_map morph_fn r) (lang_fn l).
+    Proof.
+      elim: l; auto.
+      move => a l IH; case.
+      move => -> //=; auto.
+      move => inr.
+      simpl.
+      right.
+      auto.
+    Qed.
+
+    Lemma morph_lookup s n
+      : morph_fn (var_lookup s n) = var_lookup (List.map morph_fn s) n.
+    Proof.
+      elim: s n; simpl; auto.
+      move => e s' IH.
+      case; auto.
+    Qed.
+
+    Lemma morph_alg_comm n s v s'
+      : (morph_alg (ccon s v)) [/ s' /]
+        = morph_alg (@ccon _ _ n s (Vector.map (exp_subst^~ s') v)).
+    Proof.
+      unfold morph_alg.
+      unfold id_alg.
+      (*Issue: this is a sort of paramentricity here! (bad)
+        the best thing is probably to do as I did before and construct an initial
+        representation.
+        Allowed operations:
+        - intuitionistic treatment of subterms (dropping, swapping, duplicating)
+        - functions over coefficients
+       *)          
+      simpl.
+      elim: p1 p2 n s v s'.
+      
+    Lemma morph_sub_comm e s
+      : morph_fn (e[/s/]) = (morph_fn e)[/List.map morph_fn s/].
+    Proof.
+      elim: e; simpl; auto.
+      - by apply: morph_lookup.
+      - intros.
+        unfold morph_fn.
+        simpl.
+       
+      
+      elim: s; simpl; auto.
+      rewrite !empty_subst_id => //=.
+      move => a l.
+      Admitted.
+    
+    (*TODO: reformulate using a def of preservation? *)
+    (*NOTE!!! Assuming this is true, and it should be,
+      it gives a generic definition of the image of a translation,
+      i.e. target terms that are correspond to well-structured source terms
+      Suffices to show that wf_transport (source l) x ->wf  (target l) x?
+      I.e. every morphism gives rise to an equivalence preserving compiler
+     *)
+    Lemma wf_transport
+      : (forall (l : lang p1) c1 c2 t1 t2,
+            le_sort l c1 c2 t1 t2 ->
+            le_sort (lang_fn l) (ctx_fn c1) (ctx_fn c2) (morph_fn t1) (morph_fn t2))
+        /\ (forall (l : lang p1) c1 c2 s1 s2 c1' c2',
+               le_subst l c1 c2 s1 s2 c1' c2' ->
+               le_subst (lang_fn l)
+                        (ctx_fn c1) (ctx_fn c2)
+                        (List.map morph_fn s1) (List.map morph_fn s2)
+                        (ctx_fn c1') (ctx_fn c2'))
+        /\ (forall (l : lang p1) c1 c2 e1 e2 t1 t2,
+               le_term l c1 c2 e1 e2 t1 t2 ->
+               le_term (lang_fn l)
+                       (ctx_fn c1) (ctx_fn c2)
+                       (morph_fn e1) (morph_fn e2)
+                       (morph_fn t1) (morph_fn t2))
+        /\ (forall (l : lang p1) c1 c2,
+               le_ctx l c1 c2 ->
+               le_ctx (lang_fn l) (ctx_fn c1) (ctx_fn c2))
+        /\ (forall (l : lang p1) c1 c2 v1 v2,
+               le_ctx_var l c1 c2 v1 v2 ->
+               le_ctx_var (lang_fn l)
+                          (ctx_fn c1) (ctx_fn c2)
+                          (ctx_var_map morph_fn v1) (ctx_var_map morph_fn v2))
+        /\ (forall (l : lang p1) c t, 
+            wf_sort l c t ->
+            wf_sort (lang_fn l) (ctx_fn c) (morph_fn t))
+        /\ (forall (l : lang p1) c s c',
+               wf_subst l c s c' ->
+               wf_subst (lang_fn l) (ctx_fn c) (List.map morph_fn s) (ctx_fn c'))
+        /\ (forall (l : lang p1) c e t, 
+               wf_term l c e t ->
+               wf_term (lang_fn l) (ctx_fn c) (morph_fn e) (morph_fn t))
+        /\ (forall (l : lang p1) c,  wf_ctx l c -> wf_ctx (lang_fn l) (ctx_fn c))
+        /\ (forall (l : lang p1) c v,
+               wf_ctx_var l c v ->
+               wf_ctx_var (lang_fn l) (ctx_fn c) (ctx_var_map morph_fn v))
+        /\ (forall (l : lang p1) r,  wf_rule l r -> wf_rule (lang_fn l) (rule_map morph_fn r))
+        /\ (forall (l : lang p1),  wf_lang l -> wf_lang (lang_fn l)).
+    Proof.
+      apply: mono_ind'; simpl; eauto.
+      all: try by intros; rewrite !morph_sub_comm; eauto.
+      all: try by intros; (*TODO: write, use intro_to tactic *)
+        apply morph_rule_in in H1; simpl in H1;
+        auto.
+      - intros.
+        eapply le_subst_term;
+          first by auto.
+        rewrite -!morph_sub_comm; done.
+      - move => l  s c' e t t'.
+        rewrite !morph_sub_comm.
+        auto.
+    Qed.
+        (* Note!!!!: probably a theorem:
+           Derivable l r -> Preserving (r::l) -> l
+           Maybe a Thm?
+           Admissible l r -> Preserving (r::l) -> l 
+           ---- 
+           Derivable l {| c |- t} := wf_sort l c t
+           Admissible l {| c |- t} <-> wf_sort l c t ?
+         *)
     
   End MorphFns.
 
